LeanStlc/Preservation.lean
@@ -5,28 +5,28 @@ import LeanStlc.Typing
 open LeanSubst
 
 theorem preservation_step {Γ A t t'} : Γ ⊢ t : A -> t ~> t' -> Γ ⊢ t' : A := by
-intro j r
-induction j generalizing t'
-case var => cases r
-case app j1 j2 ih1 ih2 =>
-  cases r
-  case beta =>
-    cases j1; case _ j1 =>
-    apply typing_beta j1 j2
-  case app1 r =>
-    replace ih1 := ih1 r
-    apply Typing.app ih1 j2
-  case app2 r =>
-    replace ih2 := ih2 r
-    apply Typing.app j1 ih2
-case lam j ih =>
-  cases r
-  case lam r =>
-    replace ih := ih r
-    apply Typing.lam ih
+  intro j r
+  induction j generalizing t'
+  case var => cases r
+  case app j1 j2 ih1 ih2 =>
+    cases r
+    case beta =>
+      cases j1; case _ j1 =>
+      apply typing_beta j1 j2
+    case app1 r =>
+      replace ih1 := ih1 r
+      apply Typing.app ih1 j2
+    case app2 r =>
+      replace ih2 := ih2 r
+      apply Typing.app j1 ih2
+  case lam j ih =>
+    cases r
+    case lam r =>
+      replace ih := ih r
+      apply Typing.lam ih
 
 theorem preservation {Γ A t t'} : Γ ⊢ t : A -> t ~>* t' -> Γ ⊢ t' : A := by
-intro j r
-induction r
-case _ => apply j
-case _ r1 r2 ih => apply preservation_step ih r2
+  intro j r
+  induction r
+  case _ => apply j
+  case _ r1 r2 ih => apply preservation_step ih r2
