LeanStlc/Typing.lean
@@ -7,7 +7,7 @@ open LeanSubst
 inductive Typing : List Ty -> Term -> Ty -> Prop where
 | var {Γ T x} :
   Γ[x]? = .some T ->
-  Typing Γ #x T
+  Typing Γ (.var x) T
 | app {Γ A B f a} :
   Typing Γ f (A -t> B) ->
   Typing Γ a A ->
@@ -19,96 +19,96 @@ inductive Typing : List Ty -> Term -> Ty -> Prop where
 notation:170 Γ:170 " ⊢ " t:170 " : " A:170 => Typing Γ t A
 
 theorem typing_renaming_lift {Γ Δ} A {r : Ren} :
-  (∀ x T, Γ ⊢ #x : T -> Δ ⊢ #(r x) : T) ->
-  ∀ x T, (A::Γ) ⊢ #x : T -> (A::Δ) ⊢ #(r.lift x) : T
+  (∀ x T, Γ ⊢ .var x : T -> Δ ⊢ .var (r x) : T) ->
+  ∀ x T, (A::Γ) ⊢ .var x : T -> (A::Δ) ⊢ .var (r.lift x) : T
 := by
-intro h x T j
-simp [Ren.lift]; cases x <;> simp at *
-case _ =>
-  cases j; case _ j =>
-  apply Typing.var
-  simp at *; subst j; rfl
-case _ x =>
-  cases j; case _ j =>
-  simp at j; apply Typing.var
-  simp; have lem := h x T (Typing.var j)
-  cases lem; case _ lem =>
-  apply lem
+  intro h x T j
+  simp [Ren.lift]; cases x <;> simp at *
+  case _ =>
+    cases j; case _ j =>
+    apply Typing.var
+    simp at *; subst j; rfl
+  case _ x =>
+    cases j; case _ j =>
+    simp at j; apply Typing.var
+    simp; have lem := h x T (Typing.var j)
+    cases lem; case _ lem =>
+    apply lem
 
 theorem typing_weaken {Γ t A} Δ (r : Ren) :
   Γ ⊢ t : A ->
-  (∀ x T, Γ ⊢ #x : T -> Δ ⊢ #(r x) : T) ->
+  (∀ x T, Γ ⊢ .var x : T -> Δ ⊢ .var (r x) : T) ->
   Δ ⊢ Ren.apply r t : A
 := by
-intro j h
-induction j generalizing Δ r
-case var j =>
-  apply h _ _
-  apply Typing.var j
-case app j1 j2 ih1 ih2 =>
-  apply Typing.app
-  replace ih1 := ih1 _ _ h; simp at ih1
-  apply ih1
-  replace ih2 := ih2 _ _ h; simp at ih2
-  apply ih2
-case lam j ih =>
-  apply Typing.lam
-  replace ih := ih _ _ (typing_renaming_lift _ h); simp at ih
-  apply ih
+  intro j h
+  induction j generalizing Δ r
+  case var j =>
+    apply h _ _
+    apply Typing.var j
+  case app j1 j2 ih1 ih2 =>
+    apply Typing.app
+    replace ih1 := ih1 _ _ h; simp at ih1
+    apply ih1
+    replace ih2 := ih2 _ _ h; simp at ih2
+    apply ih2
+  case lam j ih =>
+    apply Typing.lam
+    replace ih := ih _ _ (typing_renaming_lift _ h); simp at ih
+    apply ih
 
 theorem typing_subst_lift {Γ Δ} A {σ : Subst Term} :
-  (∀ x T, Γ ⊢ #x : T -> Δ ⊢ ↑(σ x) : T) ->
-  ∀ x T, (A::Γ) ⊢ #x : T -> (A::Δ) ⊢ ↑(σ.lift x) : T
+  (∀ x T, Γ ⊢ .var x : T -> Δ ⊢ σ x : T) ->
+  ∀ x T, (A::Γ) ⊢ .var x : T -> (A::Δ) ⊢ σ.lift x : T
 := by
-intro h x T j
-cases j; case _ j =>
-cases x <;> simp at *
-case _ => subst j; apply Typing.var; simp
-case _ x =>
-  have h' := h _ _ (Typing.var j)
-  have lem := typing_weaken (A :: Δ) (λ x => x + 1) h' (by {
-    intro x T j2; simp
-    apply Typing.var; simp
-    cases j2; simp [*]
-  }); simp at lem
-  unfold Subst.compose; simp
-  generalize zdef : σ x = z at *
-  cases z <;> simp at *
-  apply lem
-  rw [SubstMapStable.apply_stable (σ := S) (by rw [to_S])] at lem
-  apply lem
+  intro h x T j
+  cases j; case _ j =>
+  cases x <;> simp at *
+  case _ => subst j; apply Typing.var; simp
+  case _ x =>
+    have h' := h _ _ (Typing.var j)
+    have lem := typing_weaken (A :: Δ) (λ x => x + 1) h' (by {
+      intro x T j2; simp
+      apply Typing.var; simp
+      cases j2; simp [*]
+    }); simp at lem
+    unfold Subst.compose; simp
+    generalize zdef : σ x = z at *
+    cases z <;> simp at *
+    apply lem
+    rw [SubstMapStable.apply_stable (· + 1) +1 (by rw [Ren.to_succ])] at lem
+    apply lem
 
 theorem typing_subst {Γ t A} Δ (σ : Subst Term) :
   Γ ⊢ t : A ->
-  (∀ x T, Γ ⊢ #x : T -> Δ ⊢ ↑(σ x) : T) ->
+  (∀ x T, Γ ⊢ .var x : T -> Δ ⊢ σ x : T) ->
   Δ ⊢ t[σ] : A
 := by
-intro j h
-induction j generalizing Δ σ
-case var T x j =>
-  replace h := h x T; simp
-  generalize zdef : σ x = z at *
-  cases z <;> simp at *
-  all_goals apply h; apply Typing.var j
-case app j1 j2 ih1 ih2 =>
-  simp; apply Typing.app
-  apply ih1 _ _ h
-  apply ih2 _ _ h
-case lam j ih =>
-  simp; apply Typing.lam
-  replace ih := ih _ _ (typing_subst_lift _ h)
-  simp at ih; apply ih
+  intro j h
+  induction j generalizing Δ σ
+  case var T x j =>
+    replace h := h x T; simp
+    generalize zdef : σ x = z at *
+    cases z <;> simp at *
+    all_goals apply h; apply Typing.var j
+  case app j1 j2 ih1 ih2 =>
+    simp; apply Typing.app
+    apply ih1 _ _ h
+    apply ih2 _ _ h
+  case lam j ih =>
+    simp; apply Typing.lam
+    replace ih := ih _ _ (typing_subst_lift _ h)
+    simp at ih; apply ih
 
-theorem typing_beta {Γ A B b t} : (A::Γ) ⊢ b : B -> Γ ⊢ t : A -> Γ ⊢ b[%t::I] : B := by
-intro j1 j2
-apply typing_subst Γ (%t::I) j1 (λ x T h => by {
-  simp; cases x <;> simp
-  case _ =>
-    cases h; case _ h =>
-    simp at h; subst h
-    apply j2
-  case _ x =>
-    cases h; case _ h =>
-    simp at h
-    apply Typing.var h
-})
+theorem typing_beta {Γ A B b t} : (A::Γ) ⊢ b : B -> Γ ⊢ t : A -> Γ ⊢ b[.su t::+0] : B := by
+  intro j1 j2
+  apply typing_subst Γ (.su t::+0) j1 (λ x T h => by {
+    simp; cases x <;> simp
+    case _ =>
+      cases h; case _ h =>
+      simp at h; subst h
+      apply j2
+    case _ x =>
+      cases h; case _ h =>
+      simp at h
+      apply Typing.var h
+  })
